src/FoldIn.v
@@ -1,0 +1,70 @@
+(*** List iterators that preserve evidence that each processed element belongs to the list *)
+(** Many proofs about processing keys in the [Storage.t] require some
+sort of [In k (keys s)] hypothesis. This module defines versions of
+common list processing functions that provide this hypothesis *)
+
+Require Import List.
+Import ListNotations.
+
+(** Version of list foldr that preserves evidence that key passed
+into the function is a member of the input list *)
+Definition foldl' {A B} : forall (l : list A), (forall (a : A), In a l -> B -> B) -> B -> B.
+  refine (fix foldl' l f acc0 :=
+            (match l as l0 return (l = l0 -> B) with
+             | [] => fun _ => acc0
+             | a :: t => fun Hl => foldl' t _ (f a _ acc0)
+             end) (eq_refl l)).
+  - (* Create a copy of [f] typed so it works with [t]: *)
+    intros a' Ha't acc'.
+    apply (in_cons a a' t) in Ha't.
+    rewrite <- Hl in Ha't.
+    apply (f a' Ha't acc').
+  - (* Prove that a is in l: *)
+    rewrite Hl.
+    apply in_eq.
+Defined.
+
+(** Proof of equivalence of [fold_left] with [foldl']. It can be used
+to replace one another for easier reasoning *)
+Theorem fold_left_foldl' : forall {A B} (l : list A) (f : B -> A -> B) (a : B),
+    fold_left f l a = foldl' l (fun elem HIn acc => f acc elem) a.
+Proof.
+  intros.
+  generalize dependent a.
+  induction l.
+  - easy.
+  - intros a'. simpl.
+    rewrite IHl.
+    reflexivity.
+Qed.
+
+(** Version of [forallb] that preserves the evidence that each element
+passed into the predicate function [p] is a member of the list [l] *)
+Definition forallb' {T} (l : list T) (p : forall k, In k l -> bool) :=
+  @foldl' T bool l (fun k HIn acc => andb (p k HIn) acc) true.
+
+(** Proof of equivalence of [forallb] and [forallb']. It can be used
+to replace [forallb] with [forallb'] for easier reasoning *)
+Theorem forallb_forallb' : forall {T} p (l : list T),
+    forallb p l = forallb' l (fun k HIn => p k).
+Proof.
+  intros.
+  induction l.
+  - easy.
+  - unfold forallb'. simpl.
+    rewrite IHl.
+    rewrite Bool.andb_true_r.
+    rewrite Bool.andb_comm.
+    destruct (p a).
+    + rewrite Bool.andb_true_r. reflexivity.
+    + rewrite Bool.andb_false_r.
+      { clear IHl.
+        induction l.
+        - easy.
+        - intros.
+          simpl.
+          rewrite Bool.andb_false_r.
+          rewrite <-IHl.
+          reflexivity.
+      }
+Qed.
